# 和式

## 记号

符号:$\huge\sum$

eg.
1. $a_1 + a_2 + \cdots + a_{k-1} + a_k + a_{k+1}+\cdots +a_{n-1}+a_n = \sum_{k=1}^na_k=\sum_{1\leq k \leq n} a_k$

## 成套方法
### 解决将和式转为封闭式的方法
### 前$n$个自然数的和
#### 命题

> 将$\sum_{k=1}^nk$转为封闭式

#### 求解
方法:成套方法

1. 转为递归式

令$S(n)=\sum_{k=1}^nk$
不难看出,$S(n)=S(n-1)+n$

2. 一般化

令$R(n)$为$S(n)$的一般形式
即$R(0)=\alpha \qquad R(n)=R(n-1)+\beta n+\gamma$

(1) 令$R(n)=1$

$$\therefore R(0)=1$$

$$\therefore \alpha = 1$$

$$\because R(n)=R(n-1)+\beta n+\gamma$$

$$\therefore 1=1+\beta n + \gamma$$

$$ \left\{
\begin{aligned}
\alpha = 1 \\
\beta = 0 \\
\gamma = 0
\end{aligned}
\right.
$$

(2) 令$R(n)=n$

$$\therefore R(0) = 0$$

$$\therefore \alpha = 0$$

$$\because R(n)=R(n-1)+\beta n+\gamma$$

$$\therefore n = (n-1)+\beta n + \gamma$$

$$ \left\{
\begin{aligned}
\alpha = 0 \\
\beta = 0 \\
\gamma = 1
\end{aligned}
\right.
$$

(3) 令$R(n) = n^2$

$$\therefore R(0) = 0$$

$$\therefore \alpha = 0$$

$$\because R(n)=R(n-1)+\beta n+\gamma$$

$$\therefore n^2 = (n-1)^2+\beta n + \gamma$$

$$\therefore n^2 = n^2 - 2n + 1+\beta n + \gamma$$

$$\therefore -1 =(\beta - 2) n + \gamma$$

$$ \left\{
\begin{aligned}
\alpha = 0 \\
\beta = 2 \\
\gamma = -1
\end{aligned}
\right.
$$

3.计算系数

令$R(n)=A(n)\alpha + B(n)\beta + C(n)\gamma$

(1) 当$R(n) = 1$时:

$$\because\left\{
\begin{aligned}
\alpha = 1 \\
\beta = 0 \\
\gamma = 0
\end{aligned}
\right.
$$

$$\therefore A(n) = 1$$

(2) 当$R(n) = n$时:

$$\because\left\{
\begin{aligned}
\alpha = 0 \\
\beta = 0 \\
\gamma = 1
\end{aligned}
\right.
$$

$$\therefore C(n) = n$$

(3) 当$R(n) = n^2$时:

$$ \left\{
\begin{aligned}
\alpha = 0 \\
\beta = 2 \\
\gamma = -1
\end{aligned}
\right.
$$

$$\therefore 2B(n) - C(n) = n^2$$

综上:

$$ \left\{
\begin{aligned}
A(n) = 1 \\
C(n) = n \\
2B(n) - C(n) = n^2
\end{aligned}
\right.
$$

解得

$$ \left\{
\begin{align}
A(n) = 1 \\
B(n) = \frac{n\cdot (n+1)}{2} \\
C(n) = n
\end{align}
\right.
$$

4.具体化

$$S(n) = S(n-1) + n$$

令$P(n)$为当$\beta = 1, \gamma = 0$时$R(n)$的值

$$\therefore P(n) = P(n-1) + n = S(n)$$

$\therefore S(n)$为当$\beta = 1, \gamma = 0$时$R(n)$的值

$$\therefore S(n) = B(n)$$

$$\therefore S(n) = \frac{n \cdot (n+1)}{2}$$